src/Serial.v
@@ -1,10 +1,12 @@
 Require Import Bool List String Peano_dec.
-Require Import Common ListSupport FMap Syntax Semantics StepT.
+Require Import Common ListSupport FMap Syntax Semantics StepM StepT.
 
 (** [Atomic] and [Transactional] histories *)
 
 Section PerSystem.
   Variable sys: System.
+
+  Context {MsgT} `{HasMsg MsgT}.
 
   (* A history is [Atomic] if it satisfies following conditions:
    * 1) The history can be either an incomplete or a complete transaction.
@@ -12,32 +14,30 @@ Section PerSystem.
    *    and all [hdl]s have the same [tinfo_tid]. It means that the history is
    *    for a single transaction.
    *)
-  Inductive Atomic: TrsId -> Id Msg -> THistory -> MessagePool TMsg -> Prop :=
+  Inductive Atomic: Id MsgT -> History MsgT -> MessagePool MsgT -> Prop :=
   | AtomicStart:
-      forall ts rqr rq houts,
-        Forall (fun idm => tmsg_info (valOf idm) =
-                           Some (buildTInfo ts (rq :: nil))) houts ->
-        Atomic ts rq (RlblInt (Some rqr) (liftI toTMsgU rq :: nil) houts :: nil)
+      forall rqr rq houts,
+        Atomic rq (RlblInt (Some rqr) (rq :: nil) houts :: nil)
                (enqMsgs houts (emptyMP _))
   | AtomicCont:
-      forall ts rq hst rule msgs mouts houts,
-        Atomic ts rq hst mouts ->
+      forall rq hst rule msgs mouts houts,
+        Atomic rq hst mouts ->
         msgs <> nil ->
         Forall (fun idm => InMP (idOf idm) (valOf idm) mouts) msgs ->
-        Atomic ts rq (RlblInt (Some rule) msgs houts :: hst)
+        Atomic rq (RlblInt (Some rule) msgs houts :: hst)
                (enqMsgs houts (deqMsgs (idsOf msgs) mouts)).
 
   (* A history is [ExtAtomic] iff it is [Atomic] and starts from
    * an external request.
    *)
-  Inductive ExtAtomic: TrsId -> Id Msg -> THistory -> MessagePool TMsg -> Prop :=
+  Inductive ExtAtomic: Id MsgT -> History MsgT -> MessagePool MsgT -> Prop :=
   | ExtAtomicIntro:
-      forall ts rq hst mouts,
+      forall rq hst mouts,
         In (idOf rq) (merqsOf sys) ->
-        Atomic ts rq hst mouts ->
-        ExtAtomic ts rq hst mouts.
+        Atomic rq hst mouts ->
+        ExtAtomic rq hst mouts.
 
-  Inductive Transactional: THistory -> Prop :=
+  Inductive Transactional: History MsgT -> Prop :=
   | TrsSlt:
       Transactional (emptyRLabel _ :: nil)
   | TrsIns:
@@ -49,40 +49,50 @@ Section PerSystem.
         tout = RlblOuts eouts ->
         Transactional (tout :: nil)
   | TrsAtomic:
-      forall ts rq hst mouts,
-        ExtAtomic ts rq hst mouts ->
+      forall rq hst mouts,
+        ExtAtomic rq hst mouts ->
         Transactional hst.
 
-  Definition Sequential (hst: THistory) :=
-    exists trss: list THistory,
+  Definition Sequential (hst: History MsgT) :=
+    exists trss: list (History MsgT),
       Forall Transactional trss /\
       hst = List.concat trss.
 
 End PerSystem.
 
-(** Serializability *)
+(*! Serializability *)
 
-Definition trsSteps (sys: System) (st1: TState) (hst: THistory) (st2: TState) :=
-  steps step_t sys st1 hst st2 /\
+Definition trsSteps {StateT MsgT} `{HasMsg MsgT}
+           (step: Step System StateT (RLabel MsgT))
+           (sys: System) (st1: StateT) (hst: History MsgT) (st2: StateT) :=
+  steps step sys st1 hst st2 /\
   Transactional sys hst.
 
-Definition seqSteps (sys: System) (st1: TState) (hst: THistory) (st2: TState) :=
-  steps step_t sys st1 hst st2 /\
+Definition trsStepsM := trsSteps step_m.
+Definition trsStepsT := trsSteps step_t.
+
+Definition seqSteps {StateT MsgT} `{HasMsg MsgT}
+           (step: Step System StateT (RLabel MsgT))
+           (sys: System) (st1: StateT) (hst: History MsgT) (st2: StateT) :=
+  steps step sys st1 hst st2 /\
   Sequential sys hst.
+
+Definition seqStepsM := seqSteps step_m.
+Definition seqStepsT := seqSteps step_t.
 
 Definition BEquivalent (sys: System)
            {LabelT} `{HasLabel LabelT} (ll1 ll2: list LabelT) :=
   behaviorOf sys ll1 = behaviorOf sys ll2.
 
-Definition Serializable (sys: System) (ll: THistory) :=
+Definition Serializable (sys: System) (ll: MHistory) :=
   exists sll sst,
-    (* 1) legal, 2) sequential, and *) seqSteps sys (initsOf sys) sll sst /\
+    (* 1) legal, 2) sequential, and *) seqStepsM sys (initsOf sys) sll sst /\
     (* 3) behavior-equivalent *) BEquivalent sys ll sll.
 
 (* A system is serializable when all possible behaviors are [Serializable]. *)
 Definition SerializableSys (sys: System) :=
   forall ll st,
-    steps step_t sys (initsOf sys) ll st ->
+    steps step_m sys (initsOf sys) ll st ->
     Serializable sys ll.
 
 (** Let's start (experimentally) with an obvious condition 
